[SLS] more uniform naming scheme

Weidenbach_Book/Stochastic_Local_Search/Local_Search.thy
@@ -12,7 +12,7 @@ begin
 text \<open>
 There is a technique related to SAT solving called \<^emph>\<open>local search\<close>. It involves improving a random initial assignment by flipping variables to reduce the number of unsatisfied clauses. The process starts with a random assignment and evaluates the number of unsatisfied clauses. A variable is selected (often based on its impact on unsatisfied clauses) and flipped to attempt to improve the solution. This continues until either all clauses are satisfied (a solution is found) or a stopping condition (like a maximum number of iterations) is met.
 Local search (or SLS) is not a decision procedure (in the sense that it cannot decide if the problem is unsatisfiable)
-We do not care about termination and simply want to find a model. This week we will define the calculus and next week refine it to code.
+We do not care about termination and simply want to find a model.
 \<close>
 
 
@@ -28,14 +28,13 @@ Now we define flipping: if (and only if) there is clause that is not satisfied, 
 \<close>
 inductive local_search :: \<open>'a sls_state \<Rightarrow> 'a sls_state \<Rightarrow> bool\<close>where
 
-  flip: \<open>local_search (M, N) (M - {L} \<union> {-L}, N)\<close> if \<open>C \<in># N\<close> \<open>\<not>M \<Turnstile> C\<close> and \<open>L \<in> M\<close>
+flip: \<open>local_search (M, N) (M - {L} \<union> {-L}, N)\<close> if \<open>C \<in># N\<close> \<open>\<not>M \<Turnstile> C\<close> and \<open>L \<in> M\<close>
 
 
 inductive_cases local_searchE: \<open>local_search S T\<close>
 
 text \<open>Now we define the invariants on the transition system.\<close>
 definition sls_invariant :: \<open>'a sls_state \<Rightarrow> bool\<close> where
-
   \<open>sls_invariant S = (consistent_interp (fst S) \<and> total_over_m (fst S) (set_mset (snd S)) \<and> {#} \<notin># snd S)\<close>
 
 
@@ -47,7 +46,7 @@ lemma sls_invariant_nonempty_model:
 
 lemma local_search_sls_invariant: \<open>local_search S T \<Longrightarrow> sls_invariant S \<Longrightarrow> sls_invariant T\<close>
   by (induction rule: local_search.induct)
-   (auto simp: sls_invariant_def consistent_interp_insert_iff consistent_interp_def total_over_m_def total_over_set_def)
+    (auto simp: sls_invariant_def consistent_interp_insert_iff consistent_interp_def total_over_m_def total_over_set_def)
 
 lemma rtranclp_local_search_sls_invariant: \<open>local_search\<^sup>*\<^sup>* S T \<Longrightarrow> sls_invariant S \<Longrightarrow> sls_invariant T\<close>
   by (induction rule: rtranclp_induct) (auto intro: local_search_sls_invariant)
@@ -63,7 +62,6 @@ text \<open>Now prove the correctnes theorem:\<close>
 lemma sls_final_state:
   assumes \<open>sls_invariant S\<close> and finished: \<open>\<And>T. \<not>local_search S T\<close>
   shows \<open>fst S \<Turnstile>sm (snd S)\<close>
-
 proof (rule ccontr)
   assume \<open>\<not>?thesis\<close>
   then obtain C where \<open>C \<in># snd S\<close> and \<open>\<not>fst S \<Turnstile> C\<close>
@@ -78,7 +76,7 @@ lemma sls_final_state_run:
   assumes \<open>local_search\<^sup>*\<^sup>* S T\<close> \<open>sls_invariant S\<close> and finished: \<open>\<And>U. \<not>local_search T U\<close>
   shows \<open>fst T \<Turnstile>sm (snd S)\<close>
   by (metis assms(1,2) finished rtranclp_local_search_clauses_same
-    rtranclp_local_search_sls_invariant sls_final_state)
+      rtranclp_local_search_sls_invariant sls_final_state)
 
 
 
@@ -102,135 +100,131 @@ text \<open>We define flipping again make sure that you update the multiset of b
 
 Express your definition in a way that only clauses where \<^term>\<open>L\<close> or  \<^term>\<open>-L\<close> are considered, for example with \<^term>\<open>{#C \<in># N. (L \<in># C \<and> P C)#}\<close>.
   \<close>
-inductive local_search2 :: \<open>'a sls_state2 \<Rightarrow> 'a sls_state2 \<Rightarrow> bool\<close>where
+inductive local_search_brk :: \<open>'a sls_state2 \<Rightarrow> 'a sls_state2 \<Rightarrow> bool\<close>where
+  flip: \<open>local_search_brk (M, N, br) (M - {L} \<union> {-L}, {#C \<in># N. (-L \<notin># C \<and> L \<notin># C)#} + {#C \<in># N. (-L \<in># C \<or> L \<in># C) \<and> M - {L} \<union> {-L} \<Turnstile> C#} + {#C \<in># br. (-L \<in># C)#}, br')\<close>
+if \<open>br \<noteq> {#}\<close> and \<open>L \<in> M\<close>
+  \<open>br' = {#C \<in># br. (-L \<notin># C)#} + {#C \<in># N. (L \<in># C \<and> \<not>(M - {L} \<union> {-L} \<Turnstile> C))#}\<close>
 
-  flip: \<open>local_search2 (M, N, br) (M - {L} \<union> {-L}, {#C \<in># N. (-L \<notin># C \<and> L \<notin># C)#} + {#C \<in># N. (-L \<in># C \<or> L \<in># C) \<and> M - {L} \<union> {-L} \<Turnstile> C#} + {#C \<in># br. (-L \<in># C)#}, br')\<close>
-  if \<open>br \<noteq> {#}\<close> and \<open>L \<in> M\<close>
-    \<open>br' = {#C \<in># br. (-L \<notin># C)#} + {#C \<in># N. (L \<in># C \<and> \<not>(M - {L} \<union> {-L} \<Turnstile> C))#}\<close>
 
-
-inductive_cases local_search2E: \<open>local_search2 S T\<close>
+inductive_cases local_search_brkE: \<open>local_search_brk S T\<close>
 
 fun convert_sls_state :: \<open>'a sls_state2 \<Rightarrow> 'a sls_state\<close> where
   \<open>convert_sls_state (M, N, br) = (M, N + br)\<close>
 
 
 text \<open>The new invariants:\<close>
-definition sls_invariant2 :: \<open>'a sls_state2 \<Rightarrow> bool\<close> where
-  \<open>sls_invariant2 S = (sls_invariant (convert_sls_state S) \<and> (\<forall>C\<in># broken S. \<not>fst S \<Turnstile> C) \<and> (\<forall>C\<in># sls2_clss S. fst S \<Turnstile> C))\<close>
+definition sls_invariant_brk :: \<open>'a sls_state2 \<Rightarrow> bool\<close> where
+  \<open>sls_invariant_brk S = (sls_invariant (convert_sls_state S) \<and> (\<forall>C\<in># broken S. \<not>fst S \<Turnstile> C) \<and> (\<forall>C\<in># sls2_clss S. fst S \<Turnstile> C))\<close>
 
 
-text \<open>One step by \<^term>\<open>local_search2\<close> is also a step in \<^term>\<open>local_search\<close>.\<close>
-lemma local_search2_local_search:
-  assumes \<open>local_search2 S T\<close> \<open>sls_invariant2 S\<close>
+text \<open>One step by \<^term>\<open>local_search_brk\<close> is also a step in \<^term>\<open>local_search\<close>.\<close>
+lemma local_search_brk_local_search:
+  assumes \<open>local_search_brk S T\<close> \<open>sls_invariant_brk S\<close>
   shows \<open>local_search (convert_sls_state S) (convert_sls_state T)\<close>
   using assms
-proof (induction rule: local_search2.induct)
+proof (induction rule: local_search_brk.induct)
   case (flip br L M br' N)
   let ?S = \<open>(M, N, br)\<close>
   let ?T = \<open>(M - {L} \<union> {- L},
      filter_mset ((\<Turnstile>) (M - {L} \<union> {- L})) N + filter_mset ((\<in>#) (- L)) br,
     br')\<close>
   have satis: \<open>\<And>C. C\<in># sls2_clss ?S \<Longrightarrow> fst ?S \<Turnstile> C\<close>
-    using flip by (auto simp: sls_invariant2_def)
+    using flip by (auto simp: sls_invariant_brk_def)
   have H: \<open>a \<in># N \<Longrightarrow> \<not> insert (- L) (M - {L}) \<Turnstile> a \<Longrightarrow> L \<in># a\<close> for a
     using satis[of a] by (auto simp: true_cls_def)
   have [simp]: \<open>{#C \<in># N. L \<in># C \<and> \<not> insert (- L) (M - {L}) \<Turnstile> C#} = {#C \<in># N. \<not> insert (- L) (M - {L}) \<Turnstile> C#}\<close>
     by (rule filter_mset_cong[of _ N]) (use H in auto)
-   obtain C where \<open>C \<in># br\<close> \<open>C \<in># snd (convert_sls_state ?S)\<close> and \<open>\<not>fst ?S \<Turnstile> C\<close>
-     using flip by (auto simp: sls_invariant2_def)
-   moreover have \<open> {#C \<in># N. - L \<notin># C \<and> L \<notin># C#} +
+  obtain C where \<open>C \<in># br\<close> \<open>C \<in># snd (convert_sls_state ?S)\<close> and \<open>\<not>fst ?S \<Turnstile> C\<close>
+    using flip by (auto simp: sls_invariant_brk_def)
+  moreover have \<open> {#C \<in># N. - L \<notin># C \<and> L \<notin># C#} +
      {#C \<in># N. (- L \<in># C \<or> L \<in># C) \<and> insert (- L) (M - {L}) \<Turnstile> C#} +
      filter_mset ((\<in>#) (- L)) br +
      (filter_mset ((\<notin>#) (- L)) br + {#C \<in># N. \<not> insert (- L) (M - {L}) \<Turnstile> C#}) =
      N + br\<close>
-   proof -
-     have \<open>({#C \<in># N. \<not> insert (- L) (M - {L}) \<Turnstile> C#} +
+  proof -
+    have \<open>({#C \<in># N. \<not> insert (- L) (M - {L}) \<Turnstile> C#} +
        ({#C \<in># N. L \<notin># C \<and> - L \<notin># C#} +
        {#C \<in># N. (L \<in># C \<or> - L \<in># C) \<and> insert (- L) (M - {L}) \<Turnstile> C#})) = N\<close> (is \<open>?A + (?B + ?C) = _\<close>)
-       using satis apply (induction N) apply auto by (metis atm_of_notin_atms_of_iff flip.hyps(2) insert_Diff true_cls_insert_l
-         true_cls_remove_hd_if_notin_vars)
-     moreover have \<open>filter_mset ((\<in>#) (- L)) br + filter_mset ((\<notin>#) (- L)) br + A = br + A\<close> for A by fastforce
-     ultimately show ?thesis
-       by (auto simp: ac_simps)
-   qed
-   ultimately show ?case using local_search.flip[of C \<open>snd (convert_sls_state ?S)\<close> \<open>fst ?S\<close> L] flip by auto
- qed
+      using satis apply (induction N) apply auto by (metis atm_of_notin_atms_of_iff flip.hyps(2) insert_Diff true_cls_insert_l
+          true_cls_remove_hd_if_notin_vars)
+    moreover have \<open>filter_mset ((\<in>#) (- L)) br + filter_mset ((\<notin>#) (- L)) br + A = br + A\<close> for A by fastforce
+    ultimately show ?thesis
+      by (auto simp: ac_simps)
+  qed
+  ultimately show ?case using local_search.flip[of C \<open>snd (convert_sls_state ?S)\<close> \<open>fst ?S\<close> L] flip by auto
+qed
 
 
-lemma local_search2_sls_invariant:
-  assumes \<open>local_search2 S T\<close> \<open>sls_invariant2 S\<close>
-  shows \<open>sls_invariant2 T\<close>
-  using assms local_search2_local_search[OF assms(1,2)]
-proof (induction rule: local_search2.induct)
+lemma local_search_brk_sls_invariant:
+  assumes \<open>local_search_brk S T\<close> \<open>sls_invariant_brk S\<close>
+  shows \<open>sls_invariant_brk T\<close>
+  using assms local_search_brk_local_search[OF assms(1,2)]
+proof (induction rule: local_search_brk.induct)
   case (flip br L M br' N)
   let ?T = \<open>(M - {L} \<union> {- L},{#C \<in># N. - L \<notin># C \<and> L \<notin># C#} +
      {#C \<in># N. (- L \<in># C \<or> L \<in># C) \<and> M - {L} \<union> {- L} \<Turnstile> C#} +
      filter_mset ((\<in>#) (- L)) br, br')\<close>
   have inv: \<open>sls_invariant (convert_sls_state ?T)\<close>
-    using flip local_search_sls_invariant unfolding sls_invariant2_def by blast
+    using flip local_search_sls_invariant unfolding sls_invariant_brk_def by blast
   then show ?case 
-    using flip apply (auto simp: sls_invariant2_def dest!: multi_member_split)
-    apply (metis Diff_subset Un_commute insert_def singleton_conv
-      true_cls_mono_set_mset_l true_cls_not_in_remove)
+    using flip apply (auto simp: sls_invariant_brk_def dest!: multi_member_split)
+     apply (metis Diff_subset Un_commute insert_def singleton_conv
+        true_cls_mono_set_mset_l true_cls_not_in_remove)
     by (metis atm_of_notin_atms_of_iff insert_Diff true_cls_insert_l
-      true_cls_remove_hd_if_notin_vars)
+        true_cls_remove_hd_if_notin_vars)
 qed
- 
 
-  
-lemma rtranclp_local_search2_sls_invariant:
-  assumes \<open>local_search2\<^sup>*\<^sup>* S T\<close> \<open>sls_invariant2 S\<close>
-  shows \<open>sls_invariant2 T\<close>
+lemma rtranclp_local_search_brk_sls_invariant:
+  assumes \<open>local_search_brk\<^sup>*\<^sup>* S T\<close> \<open>sls_invariant_brk S\<close>
+  shows \<open>sls_invariant_brk T\<close>
   using assms
-  by (induction rule: rtranclp_induct) (auto dest: local_search2_sls_invariant)
+  by (induction rule: rtranclp_induct) (auto dest: local_search_brk_sls_invariant)
 
-lemma rtranclp_local_search2_local_search:
-  assumes \<open>local_search2\<^sup>*\<^sup>* S T\<close> \<open>sls_invariant2 S\<close>
+lemma rtranclp_local_search_brk_local_search:
+  assumes \<open>local_search_brk\<^sup>*\<^sup>* S T\<close> \<open>sls_invariant_brk S\<close>
   shows \<open>local_search\<^sup>*\<^sup>* (convert_sls_state S) (convert_sls_state T)\<close>
-  using assms rtranclp_local_search2_sls_invariant[OF assms]
-  by (induction rule: rtranclp_induct) (auto dest: local_search2_local_search simp: local_search2_sls_invariant rtranclp_local_search2_sls_invariant)
+  using assms rtranclp_local_search_brk_sls_invariant[OF assms]
+  by (induction rule: rtranclp_induct) (auto dest: local_search_brk_local_search simp: local_search_brk_sls_invariant rtranclp_local_search_brk_sls_invariant)
 
-lemma local_search_local_search2:
-  assumes \<open>local_search (convert_sls_state S) T\<close> \<open>sls_invariant2 S\<close>
-  shows \<open>\<exists>U. local_search2 S U\<close>
+lemma local_search_local_search_brk:
+  assumes \<open>local_search (convert_sls_state S) T\<close> \<open>sls_invariant_brk S\<close>
+  shows \<open>\<exists>U. local_search_brk S U\<close>
   using assms
 proof (induction \<open>convert_sls_state S\<close> T rule: local_search.induct)
   case (flip C N M L)
   obtain unb brok where S: \<open>S = (M, unb, brok)\<close> and N: \<open>N = unb + brok\<close>
     using flip by (cases S) auto
   have \<open>brok \<noteq> {#}\<close>
-    using flip(1,2) flip(5) unfolding sls_invariant2_def S N
+    using flip(1,2) flip(5) unfolding sls_invariant_brk_def S N
     by auto
   then show ?case
-    using local_search2.intros(1)[of brok L M _ unb] flip(3) unfolding S by force
+    using local_search_brk.intros(1)[of brok L M _ unb] flip(3) unfolding S by force
 qed
 
 
 text \<open>Now prove the overall correctness theorem. You should reuse the theorem of the first part for the satisfiability, not reprove it!\<close>
-lemma full_local_search2_no_local_search:
-  assumes \<open>sls_invariant2 S\<close> \<open>(\<forall>U. \<not>local_search2 T U)\<close> \<open>rtranclp local_search2 S T\<close>
+lemma full_local_search_brk_no_local_search:
+  assumes \<open>sls_invariant_brk S\<close> \<open>(\<forall>U. \<not>local_search_brk T U)\<close> \<open>rtranclp local_search_brk S T\<close>
   shows \<open>(\<forall>U. \<not>local_search (convert_sls_state T) U)\<close> and
     \<open>fst T \<Turnstile>sm (snd (convert_sls_state S))\<close>
-
 proof -
-  have \<open>sls_invariant2 T\<close>
-    using assms(1,3) rtranclp_local_search2_sls_invariant by blast
+  have \<open>sls_invariant_brk T\<close>
+    using assms(1,3) rtranclp_local_search_brk_sls_invariant by blast
   have \<open>local_search\<^sup>*\<^sup>* (convert_sls_state S) (convert_sls_state T)\<close>
-    using assms(1,3) rtranclp_local_search2_local_search by blast
+    using assms(1,3) rtranclp_local_search_brk_local_search by blast
   moreover show \<open>(\<forall>U. \<not>local_search (convert_sls_state T) U)\<close>
   proof (rule ccontr)
     assume \<open>\<not>(\<forall>U. \<not>local_search (convert_sls_state T) U)\<close>
     then obtain U where \<open>local_search (convert_sls_state T) U\<close>
       by auto
-    then obtain U' where \<open>local_search2 T U'\<close>
-      using \<open>sls_invariant2 T\<close> local_search_local_search2 by blast
+    then obtain U' where \<open>local_search_brk T U'\<close>
+      using \<open>sls_invariant_brk T\<close> local_search_local_search_brk by blast
     then show False using assms(2) by auto
   qed
   ultimately show \<open>fst T \<Turnstile>sm (snd (convert_sls_state S))\<close>
-    by (metis  \<open>sls_invariant2 T\<close> convert_sls_state.elims fst_swap
-      rtranclp_local_search_clauses_same sls_final_state sls_invariant2_def
-      snd_conv swap_simp)
+    by (metis \<open>sls_invariant_brk T\<close> convert_sls_state.elims fst_swap
+        rtranclp_local_search_clauses_same sls_final_state sls_invariant_brk_def
+        snd_conv swap_simp)
 qed
 
 end
