Weidenbach_Book/Stochastic_Local_Search/Local_Search_Watch.thy
@@ -9,7 +9,7 @@ theory Local_Search_Watch
   imports Local_Search 
 begin
 
-text\<open>This theory defines a variant of local search (defined in Local_Search.thy) with watched literals\<close>
+text\<open>This theory defines a variant of local search with watched literals\<close>
 
 text\<open>old version: watched list as a collection (literal, multiset of clauses watched by literal) pairs
 this approach requires existential quantification\<close>
@@ -18,29 +18,26 @@ This simplifies flipping since not all clauses need to be checked and each claus
 has exactly one watched literal
 \<close>
 
-datatype 'a wclause = WC (watched_lit: \<open>'a literal\<close>) (unwatched: \<open>'a clause\<close>)
+datatype 'a single_w_cls = WC (watched_lit: \<open>'a literal\<close>) (unwatched: \<open>'a clause\<close>)
 
 text\<open>reconstructs the original clause from a watched clause by adding the watched literal back to the unwatched part (rest of clause)\<close>
-fun clause_of :: \<open>'a wclause \<Rightarrow> 'a clause\<close>  where
+fun clause_of :: \<open>'a single_w_cls \<Rightarrow> 'a clause\<close>  where
   \<open>clause_of (WC L C) = add_mset L C\<close>
 
-type_synonym 'a wclauses = \<open>'a wclause multiset\<close>
+type_synonym 'a single_w_clss = \<open>'a single_w_cls multiset\<close>
 
 (*sls_state: M, N, br*)
-type_synonym 'a sls_state_watch = \<open>'a literal set \<times> 'a wclauses \<times> 'a clauses\<close>
+type_synonym 'a sls_watch_state = \<open>'a literal set \<times> 'a single_w_clss \<times> 'a clauses\<close>
 
-abbreviation broken :: \<open>'a sls_state_watch \<Rightarrow> 'a clauses\<close> where
+abbreviation broken :: \<open>'a sls_watch_state \<Rightarrow> 'a clauses\<close> where
   \<open>broken S \<equiv> (snd (snd S))\<close>
 
-abbreviation sls2w_clss :: \<open>'a sls_state_watch \<Rightarrow> 'a wclauses\<close> where
+abbreviation sls2w_clss :: \<open>'a sls_watch_state \<Rightarrow> 'a single_w_clss\<close> where
   \<open>sls2w_clss S \<equiv> fst (snd S)\<close>
 
-abbreviation watches :: \<open>'a sls_state_watch \<Rightarrow> ('a literal \<Rightarrow> 'a wclause multiset)\<close> where
-  \<open>watches S \<equiv> \<lambda>L. {#C \<in># sls2w_clss S. L = watched_lit C#}\<close>
-
-text\<open>function for mapping a literal L to the multiset of wclauses S whose watched_lit equals L\<close>
-definition watched :: \<open>'a literal \<Rightarrow> 'a sls_state_watch \<Rightarrow> 'a wclause multiset\<close> where
-  \<open>watched L S \<equiv> watches S L\<close>
+text\<open>function for mapping a literal L to the multiset of single_w_clss S whose watched_lit equals L\<close>
+definition watched :: \<open>'a literal \<Rightarrow> 'a sls_watch_state \<Rightarrow> 'a single_w_cls multiset\<close> where
+  \<open>watched L S \<equiv> {#C \<in># sls2w_clss S. L = watched_lit C#}\<close>
 
 
 text\<open>
@@ -52,49 +49,49 @@ updating watch list:
     add clause to broken
 
 Because each clause has only one watched literal only the watched_lit is changed
-The update is local and consumes exactly one wclause -> for all watch lists use reflexive-transitive closure @{term"(update_wl L)\<^sup>*\<^sup>* "} 
+The update is local and consumes exactly one single_w_cls -> for all watch lists use reflexive-transitive closure @{term"(update_flip_watched L)\<^sup>*\<^sup>* "} 
 \<close>
-inductive update_wl :: \<open>'a literal \<Rightarrow> 'a sls_state_watch \<times> 'a wclauses \<Rightarrow>
-    'a sls_state_watch \<times> 'a wclauses \<Rightarrow> bool\<close> where
- (*C \<in> watched L and L' \<in> C \<inter> M*)
-other_true_literal:
-   \<open>L' \<in># clause_of C \<and> L' \<in> fst S \<Longrightarrow>
-     update_wl L (S, add_mset (C:: 'a wclause) WL)
+inductive update_flip_watched :: \<open>'a literal \<Rightarrow> 'a sls_watch_state \<times> 'a single_w_clss \<Rightarrow>
+    'a sls_watch_state \<times> 'a single_w_clss \<Rightarrow> bool\<close> where
+  (*C \<in> watched L and L' \<in> C \<inter> M*)
+  other_true_literal:
+  \<open>L' \<in># clause_of C \<and> L' \<in> fst S \<Longrightarrow>
+     update_flip_watched L (S, add_mset (C:: 'a single_w_cls) WL)
             ((fst S, sls2w_clss S - {#C#} + {#WC L' (remove1_mset L' (clause_of C))#}, broken S), WL)\<close>
 | (*broken clauses*)
-broken_clause:
-   \<open>(\<forall>L'. L' \<in># clause_of C \<longrightarrow> L' \<notin> fst S) \<Longrightarrow>
-     update_wl L (S, add_mset C WL)
+  broken_clause:
+  \<open>(\<forall>L'. L' \<in># clause_of C \<longrightarrow> L' \<notin> fst S) \<Longrightarrow>
+     update_flip_watched L (S, add_mset C WL)
        ((fst S, sls2w_clss S - {#C#}, add_mset (clause_of C) (broken S)), WL)\<close>
 
 
 text\<open>
 - \<forall> C \<in> br:
   if -L \<in> C: br - {#C#} and -L := {#C#} + watch -L
--Updating the watch list is done incrementally with update_wl,
+-Updating the watch list is done incrementally with update_flip_watched,
   so there is no need for a complete new computation of broken clauses or watch lists
   only local changes
 \<close>
 
-inductive local_search_watch :: \<open>'a sls_state_watch \<Rightarrow> 'a sls_state_watch \<Rightarrow> bool\<close> where
+inductive watch_local_search :: \<open>'a sls_watch_state \<Rightarrow> 'a sls_watch_state \<Rightarrow> bool\<close> where
   flip:
-    \<open>local_search_watch
+  \<open>watch_local_search
       (M, N, br)
       (M', N'', br')\<close>
-    if
-      \<open>M' = M - {L} \<union> {-L}\<close>
-      \<open>br1 = br - {#C \<in># br. -L \<in># C#}\<close>
-      \<open>N' = N + image_mset (\<lambda>C. WC (-L) (C - {#-L#})) {#C \<in># br. -L \<in># C#}\<close>
-      \<open>(update_wl L)\<^sup>*\<^sup>* ((M', N', br1), watched L (M', N', br1)) ((M', N'', br'), {#})\<close>
-      \<open>L \<in> M\<close>
-      \<open>br \<noteq> {#}\<close>
+if
+  \<open>M' = M - {L} \<union> {-L}\<close>
+  \<open>br1 = br - {#C \<in># br. -L \<in># C#}\<close>
+  \<open>N' = N + (\<lambda>C. WC (-L) (C - {#-L#})) `# {#C \<in># br. -L \<in># C#}\<close>
+  \<open>(update_flip_watched L)\<^sup>*\<^sup>* ((M', N', br1), watched L (M', N', br1)) ((M', N'', br'), {#})\<close>
+  \<open>L \<in> M\<close>
+  \<open>br \<noteq> {#}\<close>
 
 
-inductive_cases local_searchwE: \<open>local_search_watch S T\<close>
+inductive_cases local_searchwE: \<open>watch_local_search S T\<close>
 
 
-fun convert_sls_state_watch :: \<open>'a sls_state_watch \<Rightarrow> 'a sls_state\<close> where
-  \<open>convert_sls_state_watch (M, N, br) = (M, image_mset clause_of N + br)\<close>
+fun convert_sls_watch_state :: \<open>'a sls_watch_state \<Rightarrow> 'a sls_state\<close> where
+  \<open>convert_sls_watch_state (M, N, br) = (M, image_mset clause_of N + br)\<close>
 
 text\<open>
 No need for a separate invariant about literals existing in watches, since the definition always has one watched literal
@@ -107,7 +104,7 @@ The current version makes it easier to define the invariant without searching fo
 conditions:
 - all C in broken S are unsatisfied by the current model fst S
 - for every watched clause C in sls2w_clss S, the watched_lit C is present in the model fst S\<close>
-(*
+  (*
 Invariant: 
 - sls_invariant holds
 - \<Union># (watched L) = N - br (all c \<in> N \<rightarrow> one watched literal)
@@ -116,29 +113,27 @@ Invariant:
 - watch list is consistent (before and after flipping)
 *)
 
-definition sls_invariant_watch :: \<open>'a sls_state_watch \<Rightarrow> bool\<close> where
-  \<open>sls_invariant_watch S \<equiv> 
-    (sls_invariant (convert_sls_state_watch S)) \<and>
+definition sls_watch_invariant :: \<open>'a sls_watch_state \<Rightarrow> bool\<close> where
+  \<open>sls_watch_invariant S \<equiv> 
+    (sls_invariant (convert_sls_watch_state S)) \<and>
     (\<forall>C \<in># broken S. \<not>(fst S \<Turnstile> C)) \<and>
     (\<forall>C \<in># sls2w_clss S. watched_lit C \<in> fst S)
  \<close>
 
-
-
-fun convert_sls_state_watch_step :: \<open>'a sls_state_watch  \<times> 'a wclauses \<Rightarrow> 'a sls_state\<close> where
-  \<open>convert_sls_state_watch_step ((M, N, br), WL) = (M, image_mset clause_of (N) + br)\<close>
+fun convert_sls_watch_state_step :: \<open>'a sls_watch_state  \<times> 'a single_w_clss \<Rightarrow> 'a sls_state\<close> where
+  \<open>convert_sls_watch_state_step ((M, N, br), WL) = (M, image_mset clause_of (N) + br)\<close>
 
 text\<open>local invariant while processing the watch list\<close>
-fun invariant_step:: \<open> 'a literal \<Rightarrow> 'a sls_state_watch \<times> 'a wclauses \<Rightarrow> bool\<close> where
-invariant_step_def[simp del]:\<open>invariant_step L (S, WL) \<longleftrightarrow>
-    (sls_invariant (convert_sls_state_watch_step (S,WL))) \<and>
+fun invariant_flipping:: \<open> 'a literal \<Rightarrow> 'a sls_watch_state \<times> 'a single_w_clss \<Rightarrow> bool\<close> where
+  invariant_flipping_def[simp del]:\<open>invariant_flipping L (S, WL) \<longleftrightarrow>
+    (sls_invariant (convert_sls_watch_state_step (S,WL))) \<and>
     (\<forall>C \<in># sls2w_clss S - WL. watched_lit C \<in> fst S) \<and>
     (\<forall>C \<in>#  WL. watched_lit C = L) \<and>
     (\<forall>C \<in># broken S. \<not>(fst S \<Turnstile> C)) \<and> 
      WL \<subseteq># sls2w_clss S \<and> 
     -L \<in> fst S
  \<close>
-(*broken updated before*)
+  (*broken updated before*)
 
 lemma helper: \<open> N +A  -
                {#Ca \<in># N. watched_lit C = watched_lit Ca#} =
@@ -146,44 +141,44 @@ lemma helper: \<open> N +A  -
   by (metis mset_remove_filtered mset_subset_eq_multiset_union_diff_commute
       multiset_filter_subset)
 
-lemma sls_invariant_watch_fststep_update_wl:
-  assumes \<open>sls_invariant_watch (M, N, br)\<close> 
-      \<open>L \<in> M\<close>
-      \<open>br \<noteq> {#}\<close>
-    shows \<open>invariant_step L ((M - {L} \<union> {-L},
+lemma sls_watch_invariant_fststep_update_flip_watched:
+  assumes \<open>sls_watch_invariant (M, N, br)\<close> 
+    \<open>L \<in> M\<close>
+    \<open>br \<noteq> {#}\<close>
+  shows \<open>invariant_flipping L ((M - {L} \<union> {-L},
            N+ image_mset (\<lambda>C. WC (-L) (C - {#-L#})) {#C \<in>#br. -L \<in># C#}, 
          br - {#C \<in># br. -L \<in># C#}), 
-      watched L (M,N,br))\<close> (is \<open>invariant_step L ((?M, ?N, ?br), ?W)\<close>)
-  using assms apply (auto simp: helper mset_remove_filtered sls_invariant_watch_def invariant_step_def watched_def)
-  defer
-  apply (simp add: true_cls_def)
-  apply fastforce
-  apply (metis uminus_not_id' wclause.sel(1))
-  apply (metis Diff_subset Un_insert_right sup_bot.right_neutral true_cls_mono_set_mset_l
+      watched L (M,N,br))\<close> (is \<open>invariant_flipping L ((?M, ?N, ?br), ?W)\<close>)
+  using assms apply (auto simp: helper mset_remove_filtered sls_watch_invariant_def invariant_flipping_def watched_def)
+      defer
+      apply (simp add: true_cls_def)
+      apply fastforce
+     apply (metis uminus_not_id' single_w_cls.sel(1))
+    apply (metis Diff_subset Un_insert_right sup_bot.right_neutral true_cls_mono_set_mset_l
       true_cls_not_in_remove)
-  apply (simp add: subset_mset.add_increasing2)
+   apply (simp add: subset_mset.add_increasing2)
   apply (auto simp: sls_invariant_def)
-  apply (metis DiffD2 consistent_interp_insert_iff insert_Diff singleton_iff uminus_of_uminus_id)
-  apply (metis atm_of_uminus atms_of_s_insert insert_Diff total_over_m_alt_def)
-    apply (auto simp: total_over_m_def total_over_set_def uminus_lit_swap atms_of_ms_def)
+     apply (metis DiffD2 consistent_interp_insert_iff insert_Diff singleton_iff uminus_of_uminus_id)
+    apply (metis atm_of_uminus atms_of_s_insert insert_Diff total_over_m_alt_def)
+   apply (auto simp: total_over_m_def total_over_set_def uminus_lit_swap atms_of_ms_def)
   done
 
 
-lemma sls_invariant_watch_nostep_update_wl:
-  assumes \<open>invariant_step L (S, {#})\<close>
-  shows \<open>sls_invariant_watch S\<close>
-  using assms unfolding invariant_step_def sls_invariant_watch_def by (cases S) auto
+lemma sls_watch_invariant_nostep_update_flip_watched:
+  assumes \<open>invariant_flipping L (S, {#})\<close>
+  shows \<open>sls_watch_invariant S\<close>
+  using assms unfolding invariant_flipping_def sls_watch_invariant_def by (cases S) auto
 
 
-lemma sls_invariant_watch_update_wl:
-  assumes  \<open>update_wl L S S'\<close> \<open>invariant_step L S\<close>
-  shows \<open>invariant_step L S'\<close> using assms
-proof (induction rule: update_wl.induct)
+lemma sls_watch_invariant_update_flip_watched:
+  assumes  \<open>update_flip_watched L S S'\<close> \<open>invariant_flipping L S\<close>
+  shows \<open>invariant_flipping L S'\<close> using assms
+proof (induction rule: update_flip_watched.induct)
   case (other_true_literal L' C S L WL)
   have [simp]: \<open>add_mset (clause_of C) 
        (clause_of `# remove1_mset C (sls2w_clss S) + Local_Search_Watch.broken S) =
      clause_of `# sls2w_clss S + Local_Search_Watch.broken S\<close>
-    by (metis (no_types, lifting) Local_Search_Watch.invariant_step_def add_mset_remove_trivial_iff insert_subset_eq_iff
+    by (metis (no_types, lifting) Local_Search_Watch.invariant_flipping_def add_mset_remove_trivial_iff insert_subset_eq_iff
         msed_map_invL other_true_literal.prems union_mset_add_mset_left)
   have H: \<open>Ca \<in># add_mset (WC L' (remove1_mset L' (clause_of C))) (remove1_mset C (sls2w_clss S)) - WL ==>
        Ca = WC L' (remove1_mset L' (clause_of C)) \<or>
@@ -192,97 +187,96 @@ proof (induction rule: update_wl.induct)
     by (metis (no_types, opaque_lifting) add_mset_diff_bothsides cancel_ab_semigroup_add_class.diff_right_commute
         comm_monoid_add_class.add_0 diff_diff_add_mset in_remove1_mset_neq)
   then show ?case
-    using other_true_literal apply (auto simp: invariant_step_def)
-
-      apply (metis convert_sls_state_watch_step.simps surjective_pairing)
+    using other_true_literal apply (auto simp: invariant_flipping_def)
+      apply (metis convert_sls_watch_state_step.simps surjective_pairing)
      apply (auto dest!: H)[]
     by (metis insert_subset_eq_iff subset_mset_imp_subset_add_mset)
-
 next
   case (broken_clause C S L WL)
-    have [simp]: \<open>Ca \<in># sls2w_clss S - WL \<longleftrightarrow> Ca\<in># sls2w_clss S - add_mset C WL \<or> Ca = C\<close> for Ca
-      by (smt (verit, ccfv_threshold) Local_Search_Watch.invariant_step_def add_mset_add_single broken_clause.prems
-          diff_diff_add_mset diff_le_mono2_mset diff_union_cancelL in_diffD in_remove1_msetI insert_DiffM
-          insert_subset_eq_iff)
+  have [simp]: \<open>Ca \<in># sls2w_clss S - WL \<longleftrightarrow> Ca\<in># sls2w_clss S - add_mset C WL \<or> Ca = C\<close> for Ca
+    by (smt (verit, ccfv_threshold) Local_Search_Watch.invariant_flipping_def add_mset_add_single broken_clause.prems
+        diff_diff_add_mset diff_le_mono2_mset diff_union_cancelL in_diffD in_remove1_msetI insert_DiffM
+        insert_subset_eq_iff)
   have \<open>sls_invariant (fst S, add_mset (clause_of C) (clause_of `#remove1_mset C (sls2w_clss S) + Local_Search_Watch.broken S))\<close>
-    using broken_clause apply (cases S)apply (auto simp: sls_invariant_def invariant_step_def)
-    apply (metis insert_image mset_subset_eq_insertD total_over_m_insert)
-    apply (metis (no_types, lifting) image_insert insert_DiffM insert_subset_eq_iff set_mset_add_mset_insert
+    using broken_clause apply (cases S)apply (auto simp: sls_invariant_def invariant_flipping_def)
+      apply (metis insert_image mset_subset_eq_insertD total_over_m_insert)
+     apply (metis (no_types, lifting) image_insert insert_DiffM insert_subset_eq_iff set_mset_add_mset_insert
         total_over_m_insert)
     by (metis image_eqI in_diffD)
-  then show ?case using broken_clause apply (auto simp: invariant_step_def)
-    apply (meson true_cls_def true_lit_def)
+  then show ?case using broken_clause apply (auto simp: invariant_flipping_def)
+     apply (meson true_cls_def true_lit_def)
     by (meson insert_subset_eq_iff)
 qed
 
 
-lemma rtranclp_sls_invariant_watch_update_wl:
-  assumes  \<open>(update_wl L)\<^sup>*\<^sup>* S S'\<close> \<open>invariant_step L S\<close>
-  shows \<open>invariant_step L S'\<close> using assms
-  by (induction rule: rtranclp_induct) (auto dest: sls_invariant_watch_update_wl)
+lemma rtranclp_sls_watch_invariant_update_flip_watched:
+  assumes  \<open>(update_flip_watched L)\<^sup>*\<^sup>* S S'\<close> \<open>invariant_flipping L S\<close>
+  shows \<open>invariant_flipping L S'\<close> using assms
+  by (induction rule: rtranclp_induct) (auto dest: sls_watch_invariant_update_flip_watched)
 
-lemma local_search_watch_sls_invariant_watch:
-  assumes \<open>local_search_watch S T\<close> and \<open>sls_invariant_watch S\<close>
-  shows \<open>sls_invariant_watch T\<close>
-using assms proof (induction rule: local_search_watch.induct)
+lemma watch_local_search_sls_watch_invariant:
+  assumes \<open>watch_local_search S T\<close> and \<open>sls_watch_invariant S\<close>
+  shows \<open>sls_watch_invariant T\<close>
+  using assms
+proof (induction rule: watch_local_search.induct)
   case (flip  M' M L br1 br N' N N'' br')
-  have start: \<open>sls_invariant_watch (M, N, br)\<close> using flip by simp 
-  have step1: \<open>invariant_step L ((M', N', br1), watched L (M, N, br))\<close> 
-    using sls_invariant_watch_fststep_update_wl[OF start, of L]
+  have start: \<open>sls_watch_invariant (M, N, br)\<close> using flip by simp 
+  have step1: \<open>invariant_flipping L ((M', N', br1), watched L (M, N, br))\<close> 
+    using sls_watch_invariant_fststep_update_flip_watched[OF start, of L]
     by (auto simp: flip)
   have WLMM': \<open>watched L (M, N, br) = watched L (M', N', br1)\<close>
     by (auto simp: flip watched_def filter_mset_empty_conv)
-  have step2: \<open>(update_wl L)\<^sup>*\<^sup>* ((M', N', br1), watched L (M', N', br1))
+  have step2: \<open>(update_flip_watched L)\<^sup>*\<^sup>* ((M', N', br1), watched L (M', N', br1))
          ((M', N'', br'), {#})\<close>
     using flip.hyps(4) by auto
-  have step3: \<open>invariant_step L ((M', N'', br'), {#})\<close>
-    using step1 rtranclp_sls_invariant_watch_update_wl[OF step2] unfolding WLMM'
+  have step3: \<open>invariant_flipping L ((M', N'', br'), {#})\<close>
+    using step1 rtranclp_sls_watch_invariant_update_flip_watched[OF step2] unfolding WLMM'
     by blast
   then show ?case
-    using sls_invariant_watch_nostep_update_wl by blast
+    using sls_watch_invariant_nostep_update_flip_watched by blast
 qed
 
 
 lemma clause_equiv:
-  assumes \<open>(update_wl L)\<^sup>*\<^sup>* S T\<close> and \<open>invariant_step L S\<close>
+  assumes \<open>(update_flip_watched L)\<^sup>*\<^sup>* S T\<close> and \<open>invariant_flipping L S\<close>
   shows \<open>clause_of `# sls2w_clss (fst S) + broken (fst S) = clause_of `# sls2w_clss (fst T) + broken (fst T)\<close>
-  using assms  proof (induction rule: rtranclp_induct)
+  using assms proof (induction rule: rtranclp_induct)
   case base
   then show ?case by auto
 next
   case (step y z)
   then show ?case
     by (smt (verit, ccfv_threshold) Groups.add_ac(2)
-        Local_Search_Watch.invariant_step_def
+        Local_Search_Watch.invariant_flipping_def
         add_mset_add_single add_mset_remove_trivial_If
         clause_of.simps fst_conv image_mset_add_mset
         insert_subset_eq_iff prod.sel(2)
-        rtranclp_sls_invariant_watch_update_wl
-        union_mset_add_mset_right update_wl.simps) 
+        rtranclp_sls_watch_invariant_update_flip_watched
+        union_mset_add_mset_right update_flip_watched.simps) 
 qed
 
 
-lemma local_search_watch_local_search:
-  assumes \<open>local_search_watch S T\<close> and \<open>sls_invariant_watch S\<close>
-  shows \<open>local_search (convert_sls_state_watch S) (convert_sls_state_watch T)\<close>
-using assms proof (induction rule: local_search_watch.induct)
+lemma watch_local_search_local_search:
+  assumes \<open>watch_local_search S T\<close> and \<open>sls_watch_invariant S\<close>
+  shows \<open>local_search (convert_sls_watch_state S) (convert_sls_watch_state T)\<close>
+  using assms proof (induction rule: watch_local_search.induct)
   case (flip M' M L br1 br N' N N'' br')
   have \<open> {#add_mset (- L) (remove1_mset (- L) x). x \<in># filter_mset ((\<in>#) (- L)) br#} = filter_mset ((\<in>#) (- L)) br\<close>
     by (metis (lifting) filter_mset_eq_add_msetD' insert_DiffM multiset.map_ident_strong)
   then have new_N: \<open>clause_of `# N + br = clause_of `# N' + br1\<close> using flip by auto
 
-  have \<open>invariant_step L ((M', N', br1), watched L (M', N', br1))\<close>
-     proof -
-       have \<open>watched L (M', N', br1) = watched L (M, N, br)\<close> 
-         by (auto simp: flip watched_def filter_mset_empty_conv)
-       have sls_inv: \<open>sls_invariant_watch (M, N, br)\<close>
-         by (simp add: flip.prems)
-       have L_in_M: \<open>L \<in> M\<close> using flip by simp
-       have br_not_empty: \<open>br \<noteq> {#}\<close> using flip by simp
-       show ?thesis
-    using sls_invariant_watch_fststep_update_wl[OF sls_inv L_in_M br_not_empty] flip
-    using \<open>watched L (M', N', br1) = watched L (M, N, br)\<close> by presburger
-    qed
+  have \<open>invariant_flipping L ((M', N', br1), watched L (M', N', br1))\<close>
+  proof -
+    have \<open>watched L (M', N', br1) = watched L (M, N, br)\<close> 
+      by (auto simp: flip watched_def filter_mset_empty_conv)
+    have sls_inv: \<open>sls_watch_invariant (M, N, br)\<close>
+      by (simp add: flip.prems)
+    have L_in_M: \<open>L \<in> M\<close> using flip by simp
+    have br_not_empty: \<open>br \<noteq> {#}\<close> using flip by simp
+    show ?thesis
+      using sls_watch_invariant_fststep_update_flip_watched[OF sls_inv L_in_M br_not_empty] flip
+      using \<open>watched L (M', N', br1) = watched L (M, N, br)\<close> by presburger
+  qed
   then have \<open>clause_of `# N' + br1 = clause_of `# N'' + br'\<close>
     using clause_equiv[of L \<open>((M', N', br1), watched L (M', N', br1))\<close> \<open>((M', N'', br'), {#})\<close>]
     using flip(4) by auto
@@ -290,31 +284,31 @@ using assms proof (induction rule: local_search_watch.induct)
     using flip
     using new_N by blast 
   obtain C where  \<open>C \<in># clause_of `# N + br\<close> \<open>\<not>M \<Turnstile> C\<close>
-    using cancel_comm_monoid_add_class.diff_cancel diff_union_cancelL flip.hyps(6) flip.prems fst_conv sls_invariant_watch_def by fastforce
+    using cancel_comm_monoid_add_class.diff_cancel diff_union_cancelL flip.hyps(6) flip.prems fst_conv sls_watch_invariant_def by fastforce
   then show ?case
-    by (metis calculation convert_sls_state_watch.simps flip.hyps(1,5) local_search.intros new_N)
+    by (metis calculation convert_sls_watch_state.simps flip.hyps(1,5) local_search.intros new_N)
 qed
 
 
-lemma rtranclp_local_search_watch_local_search:
-  assumes \<open>local_search_watch\<^sup>*\<^sup>* S T\<close> and \<open>sls_invariant_watch S\<close>
-  shows \<open>local_search\<^sup>*\<^sup>* (convert_sls_state_watch S) (convert_sls_state_watch T)\<close>
+lemma rtranclp_watch_local_search_local_search:
+  assumes \<open>watch_local_search\<^sup>*\<^sup>* S T\<close> and \<open>sls_watch_invariant S\<close>
+  shows \<open>local_search\<^sup>*\<^sup>* (convert_sls_watch_state S) (convert_sls_watch_state T)\<close>
   using assms apply (induction rule: rtranclp_induct) apply simp
-  by (smt (verit, best) local_search_watch_local_search local_search_watch_sls_invariant_watch
+  by (smt (verit, best) watch_local_search_local_search watch_local_search_sls_watch_invariant
       rtranclp.simps rtranclp_induct)
 
-lemma local_search_watch_cannot_be_stuck:
-  assumes \<open>broken S \<noteq> {#}\<close> and \<open>sls_invariant_watch S\<close>
-  shows \<open>\<exists>T. local_search_watch S T\<close>
+lemma watch_local_search_cannot_be_stuck:
+  assumes \<open>broken S \<noteq> {#}\<close> and \<open>sls_watch_invariant S\<close>
+  shows \<open>\<exists>T. watch_local_search S T\<close>
 proof -            
   obtain L where \<open>L \<in> fst S\<close>
-    using assms apply (cases S; cases \<open>broken S\<close>; auto simp: sls_invariant_watch_def sls_invariant_def)
+    using assms apply (cases S; cases \<open>broken S\<close>; auto simp: sls_watch_invariant_def sls_invariant_def)
     by (meson atm_of_notin_atms_of_iff multiset_nonemptyE total_over_set_def)
   define M' br1 N' where def:
-      \<open>M' = fst S - {L} \<union> {-L}\<close>
-      \<open>br1 = broken S - {#C \<in># broken S. -L \<in># C#}\<close>
-      \<open>N' = sls2w_clss S + image_mset (\<lambda>C. WC (-L) (C - {#-L#})) {#C \<in># broken S. -L \<in># C#}\<close>
-  have \<open>\<exists>N'' br'. (update_wl L)\<^sup>*\<^sup>* ((M', N', br1), WL) ((M', N'', br'), {#})\<close> for WL
+    \<open>M' = fst S - {L} \<union> {-L}\<close>
+    \<open>br1 = broken S - {#C \<in># broken S. -L \<in># C#}\<close>
+    \<open>N' = sls2w_clss S + image_mset (\<lambda>C. WC (-L) (C - {#-L#})) {#C \<in># broken S. -L \<in># C#}\<close>
+  have \<open>\<exists>N'' br'. (update_flip_watched L)\<^sup>*\<^sup>* ((M', N', br1), WL) ((M', N'', br'), {#})\<close> for WL
   proof (induction WL arbitrary: M' N' br1)
     case empty
     then show ?case by auto
@@ -322,47 +316,47 @@ proof -
     case (add x WL)
     then show ?case
     proof -
-      have "\<exists>m p ma. update_wl L ((M', N', br1), add_mset x WL) p \<and> (update_wl L)\<^sup>*\<^sup>* p ((M', ma, m), {#})"
+      have "\<exists>m p ma. update_flip_watched L ((M', N', br1), add_mset x WL) p \<and> (update_flip_watched L)\<^sup>*\<^sup>* p ((M', ma, m), {#})"
         by (metis add broken_clause fstI other_true_literal)
       then show ?thesis
         by (meson converse_rtranclp_into_rtranclp)
     qed
   qed
-  then show ?thesis using local_search_watch.flip[of M' \<open>fst S\<close> L br1 \<open>broken S\<close>
+  then show ?thesis using watch_local_search.flip[of M' \<open>fst S\<close> L br1 \<open>broken S\<close>
         N' \<open>sls2w_clss S\<close>] unfolding def[symmetric]
     by (metis \<open>L \<in> fst S\<close> assms(1) prod.exhaust_sel)
 qed
 
-lemma nostep_local_search_watch_no_step_local_search:
-  assumes \<open>\<And>T. \<not>local_search_watch S T\<close> and \<open>sls_invariant_watch S\<close>
-  shows \<open>\<And>T. \<not>local_search (convert_sls_state_watch S) T\<close>
-   proof -
-  have \<open>broken S = {#}\<close> using local_search_watch_cannot_be_stuck[of S]
+lemma nostep_watch_local_search_no_step_local_search:
+  assumes \<open>\<And>T. \<not>watch_local_search S T\<close> and \<open>sls_watch_invariant S\<close>
+  shows \<open>\<And>T. \<not>local_search (convert_sls_watch_state S) T\<close>
+proof -
+  have \<open>broken S = {#}\<close> using watch_local_search_cannot_be_stuck[of S]
     using assms(1,2) by blast
-  then have \<open>\<forall>C. C \<in># clause_of `# sls2w_clss S \<longrightarrow> (fst S \<Turnstile> C)\<close> using assms(2) apply (cases S) apply (auto simp: sls_invariant_watch_def)
-    by (metis clause_of.simps true_cls_add_mset wclause.exhaust_sel)
+  then have \<open>\<forall>C. C \<in># clause_of `# sls2w_clss S \<longrightarrow> (fst S \<Turnstile> C)\<close> using assms(2) apply (cases S) apply (auto simp: sls_watch_invariant_def)
+    by (metis clause_of.simps true_cls_add_mset single_w_cls.exhaust_sel)
 
-  show \<open>\<And>T. \<not>local_search (convert_sls_state_watch S) T\<close>
-    by (smt (verit) \<open>Local_Search_Watch.broken S = {#}\<close> \<open>\<forall>C. C \<in># clause_of `# sls2w_clss S \<longrightarrow> fst S \<Turnstile> C\<close> add_cancel_right_right convert_sls_state_watch.simps fst_conv
+  show \<open>\<And>T. \<not>local_search (convert_sls_watch_state S) T\<close>
+    by (smt (verit) \<open>Local_Search_Watch.broken S = {#}\<close> \<open>\<forall>C. C \<in># clause_of `# sls2w_clss S \<longrightarrow> fst S \<Turnstile> C\<close> add_cancel_right_right convert_sls_watch_state.simps fst_conv
         local_search.simps snd_conv surjective_pairing)
 qed
 
 
-lemma rtranclp_local_search_watch_sls_invariant_watch:
-  assumes \<open>local_search_watch\<^sup>*\<^sup>* S T\<close> and \<open>sls_invariant_watch S\<close>
-  shows \<open>sls_invariant_watch T\<close>
+lemma rtranclp_watch_local_search_sls_watch_invariant:
+  assumes \<open>watch_local_search\<^sup>*\<^sup>* S T\<close> and \<open>sls_watch_invariant S\<close>
+  shows \<open>sls_watch_invariant T\<close>
   using assms 
-  by (induction rule: rtranclp_induct) (auto dest: local_search_watch_sls_invariant_watch)
+  by (induction rule: rtranclp_induct) (auto dest: watch_local_search_sls_watch_invariant)
 
 lemma sls_final_state_run_watch:
-  assumes \<open>local_search_watch\<^sup>*\<^sup>* S T\<close> \<open>sls_invariant_watch S\<close> and finished: \<open>\<And>U. \<not>local_search_watch T U\<close>
-  shows \<open>fst (convert_sls_state_watch T) \<Turnstile>sm (snd (convert_sls_state_watch S))\<close>
-(*<*)
-  using sls_final_state_run[of \<open>convert_sls_state_watch S\<close>  \<open>convert_sls_state_watch T\<close>]
-    rtranclp_local_search_watch_local_search[OF assms(1,2)]
-    nostep_local_search_watch_no_step_local_search[OF finished]
-    rtranclp_local_search_watch_sls_invariant_watch[OF assms(1)]
-    assms(2) unfolding sls_invariant_watch_def
+  assumes \<open>watch_local_search\<^sup>*\<^sup>* S T\<close> \<open>sls_watch_invariant S\<close> and finished: \<open>\<And>U. \<not>watch_local_search T U\<close>
+  shows \<open>fst (convert_sls_watch_state T) \<Turnstile>sm (snd (convert_sls_watch_state S))\<close>
+    (*<*)
+  using sls_final_state_run[of \<open>convert_sls_watch_state S\<close>  \<open>convert_sls_watch_state T\<close>]
+    rtranclp_watch_local_search_local_search[OF assms(1,2)]
+    nostep_watch_local_search_no_step_local_search[OF finished]
+    rtranclp_watch_local_search_sls_watch_invariant[OF assms(1)]
+    assms(2) unfolding sls_watch_invariant_def
   by simp
     (*>*)
 
