Weidenbach_Book/Stochastic_Local_Search/Local_Search_Watch_List.thy
@@ -11,159 +11,158 @@ theory Local_Search_Watch_List
   imports Local_Search_Watch
 begin
 
-type_synonym 'a sls_state_watch_list = \<open>'a literal set \<times> 'a wclauses \<times> 'a clauses \<times> ('a literal \<Rightarrow> 'a wclause multiset)\<close>
+type_synonym 'a sls_watch_state_list = \<open>'a literal set \<times> 'a single_w_clss \<times> 'a clauses \<times> ('a literal \<Rightarrow> 'a single_w_cls multiset)\<close>
 
 
 
-abbreviation broken :: \<open>'a sls_state_watch_list \<Rightarrow> 'a clauses\<close> where
+abbreviation broken :: \<open>'a sls_watch_state_list \<Rightarrow> 'a clauses\<close> where
   \<open>broken S \<equiv> fst (snd (snd S))\<close>
 
-abbreviation sls2w_clss :: \<open>'a sls_state_watch_list \<Rightarrow> 'a wclauses\<close> where
+abbreviation sls2w_clss :: \<open>'a sls_watch_state_list \<Rightarrow> 'a single_w_clss\<close> where
   \<open>sls2w_clss S \<equiv> fst (snd S)\<close>
 
-abbreviation watch :: \<open>'a sls_state_watch_list \<Rightarrow> ('a literal \<Rightarrow> 'a wclause multiset)\<close> where
+abbreviation watch :: \<open>'a sls_watch_state_list \<Rightarrow> ('a literal \<Rightarrow> 'a single_w_cls multiset)\<close> where
   \<open>watch S \<equiv> snd (snd (snd S))\<close>
 
 
-fun convert_sls_state_watch_list :: \<open>'a sls_state_watch_list \<Rightarrow> 'a sls_state_watch\<close> where
-  \<open>convert_sls_state_watch_list (M, N, br, wl) = (M, N, br)\<close>
+fun convert_sls_watch_state_list :: \<open>'a sls_watch_state_list \<Rightarrow> 'a sls_watch_state\<close> where
+  \<open>convert_sls_watch_state_list (M, N, br, wl) = (M, N, br)\<close>
 
 
-definition sls_invariant_watch_list :: \<open>'a sls_state_watch_list \<Rightarrow> bool\<close> where
-  \<open>sls_invariant_watch_list S \<equiv> 
-    (sls_invariant_watch (convert_sls_state_watch_list S)) \<and>
-  watch S = watches (convert_sls_state_watch_list S)
+definition sls_watch_invariant_list :: \<open>'a sls_watch_state_list \<Rightarrow> bool\<close> where
+  \<open>sls_watch_invariant_list S \<equiv> 
+    (sls_watch_invariant (convert_sls_watch_state_list S)) \<and>
+  watch S = (\<lambda>L. watched L (convert_sls_watch_state_list S))\<close>
+
+definition invariant_wl_flipping :: \<open>'a literal \<Rightarrow> 'a sls_watch_state_list \<Rightarrow> bool\<close> where
+  \<open>invariant_wl_flipping L S \<equiv> 
+    (invariant_flipping L (convert_sls_watch_state_list S, watch S L)) \<and>
+    (watch S) = (\<lambda>L. watched L (convert_sls_watch_state_list S))
   \<close>
 
-definition invariant_wl_step :: \<open>'a sls_state_watch_list \<Rightarrow> 'a literal \<Rightarrow> bool\<close> where
-  \<open>invariant_wl_step S L \<equiv> 
-    (invariant_step L (convert_sls_state_watch_list S, watch S L)) \<and>
-    (watch S) = watches (convert_sls_state_watch_list S)
-  \<close>
 
-
-inductive update_wl_list :: \<open>'a literal \<Rightarrow> 'a sls_state_watch_list  \<Rightarrow>
-    'a sls_state_watch_list  \<Rightarrow> bool\<close> where
-  (*C \<in> watched L and L' \<in> C \<inter> M*)
-  other_true_literal:
-  \<open>L' \<in># clause_of C \<and> L' \<in> M \<Longrightarrow> WL L =  add_mset (C:: 'a wclause) WL_remaining \<Longrightarrow>
-     update_wl_list L (M, N, br, WL)
+inductive update_flip_watched_list :: \<open>'a literal \<Rightarrow> 'a sls_watch_state_list  \<Rightarrow>
+    'a sls_watch_state_list  \<Rightarrow> bool\<close> where
+other_true_literal:
+  \<open>L' \<in># clause_of C \<and> L' \<in> M \<Longrightarrow> WL L =  add_mset (C:: 'a single_w_cls) WL_remaining \<Longrightarrow>
+     update_flip_watched_list L (M, N, br, WL)
             (M, N - {#C#} + {#WC L' (remove1_mset L' (clause_of C))#}, br, 
-  WL(L:= WL_remaining, L' := WL L' + {#WC L' (remove1_mset L' (clause_of C))#}))\<close>
-| (*broken clauses*)
-  broken_clause:
-  \<open>(\<forall>L'. L' \<in># clause_of C \<longrightarrow> L' \<notin> M) \<Longrightarrow>  WL L = add_mset (C::'a wclause) WL_remaining \<Longrightarrow>
-     update_wl_list L (M, N, br, WL)
+  WL(L:= WL_remaining, L' := WL L' + {#WC L' (remove1_mset L' (clause_of C))#}))\<close> |
+broken_clause:
+  \<open>(\<forall>L'. L' \<in># clause_of C \<longrightarrow> L' \<notin> M) \<Longrightarrow>  WL L = add_mset (C::'a single_w_cls) WL_remaining \<Longrightarrow>
+     update_flip_watched_list L (M, N, br, WL)
        (M, N - {#C#}, add_mset (clause_of C) (br), WL(L:= WL_remaining))\<close>
 
 
-text\<open>calculating WL1 instead of updating with update_wl_list for simplicity\<close>
-inductive local_search_watch_list :: \<open>'a sls_state_watch_list \<Rightarrow> 'a sls_state_watch_list \<Rightarrow> bool\<close> where
+text\<open>calculating WL1 instead of updating with update_flip_watched_list for simplicity\<close>
+inductive watch_local_search_list :: \<open>'a sls_watch_state_list \<Rightarrow> 'a sls_watch_state_list \<Rightarrow> bool\<close> where
   flip:
-  \<open>local_search_watch_list
+  \<open>watch_local_search_list
       (M, N, br, WL)
       (M', N'', br', WL')\<close>
 if
   \<open>M' = M - {L} \<union> {-L}\<close>
   \<open>br1 = br - {#C \<in># br. -L \<in># C#}\<close>
   \<open>N' = N + image_mset (\<lambda>C. WC (-L) (C - {#-L#})) {#C \<in># br. -L \<in># C#}\<close>
-  \<open>WL1 = watches(M, N', br)\<close> 
-  \<open>(update_wl_list L)\<^sup>*\<^sup>* (M', N', br1, WL1) (M', N'', br', WL')\<close>
+  \<open>WL1 = (\<lambda>L. watched L (M, N', br))\<close> 
+  \<open>(update_flip_watched_list L)\<^sup>*\<^sup>* (M', N', br1, WL1) (M', N'', br', WL')\<close>
   \<open>L \<in> M\<close>
   \<open>br \<noteq> {#}\<close>
   \<open>WL' L = {#}\<close>
 
 
 lemma watch_list_eq:
-  assumes \<open>update_wl_list L (M,N,br,WL) (M',N',br',WL')\<close>
-    and \<open>invariant_wl_step (M,N,br,WL) L\<close>
-  shows   \<open>update_wl L ((M, N, br), WL L) ((M', N', br'), WL' L)\<close>
+  assumes
+    \<open>update_flip_watched_list L (M,N,br,WL) (M',N',br',WL')\<close> and
+    \<open>invariant_wl_flipping L (M,N,br,WL)\<close>
+  shows \<open>update_flip_watched L ((M, N, br), WL L) ((M', N', br'), WL' L)\<close>
   using assms proof cases
   case (other_true_literal L' C WL_remaining)
   have \<open>L \<noteq> L'\<close>
-    by (metis Local_Search_Watch.invariant_step_def assms(2) consistent_interp_insert_iff
-        convert_sls_state_watch_list.simps convert_sls_state_watch_step.simps fst_conv insert_Diff insert_iff
-        invariant_wl_step_def local.other_true_literal(5) set_mset_add_mset_insert sls_invariant_def tautology_decomp'
+    by (metis Local_Search_Watch.invariant_flipping_def assms(2) consistent_interp_insert_iff
+        convert_sls_watch_state_list.simps convert_sls_watch_state_step.simps fst_conv insert_Diff insert_iff
+        invariant_wl_flipping_def local.other_true_literal(5) set_mset_add_mset_insert sls_invariant_def tautology_decomp'
         tautology_single)
   then show ?thesis
-    by (simp add: local.other_true_literal(1,2,3,4,5,6) update_wl.simps) 
+    by (simp add: local.other_true_literal(1,2,3,4,5,6) update_flip_watched.simps) 
 next
   case (broken_clause C WL_remaining)
   then show ?thesis
-    by (simp add: update_wl.simps) 
+    by (simp add: update_flip_watched.simps) 
 qed
 
 
-lemma update_wl_list_correct:
-  assumes \<open>update_wl_list L (M,N,br,WL) (M',N',br',WL')\<close>
-    and  inv: \<open>invariant_wl_step (M,N,br,WL) L\<close>
-  shows   \<open>invariant_wl_step (M',N',br',WL') L\<close>
+lemma update_flip_watched_list_correct:
+  assumes \<open>update_flip_watched_list L S T\<close>
+    and inv: \<open>invariant_wl_flipping L S\<close>
+  shows \<open>invariant_wl_flipping L T\<close>
 proof -
-  have \<open>update_wl L ((M, N, br), WL L) ((M', N', br'), WL' L)\<close>
-    by (simp add: assms(1,2) watch_list_eq)
-  then have \<open>invariant_step L ((M', N', br'), WL' L)\<close>
-    by (metis assms(2) convert_sls_state_watch_list.simps invariant_wl_step_def
-        sls_invariant_watch_update_wl snd_eqD)
-  moreover have \<open>watch (M',N',br',WL') = watches (convert_sls_state_watch_list (M',N',br',WL'))\<close>
-    using assms
-  proof (induction rule: update_wl_list.induct)
+  obtain M N br WL M' N' br' WL' where
+   ST[simp]: \<open>S = (M,N,br,WL)\<close> \<open>T = (M',N',br',WL')\<close>
+   by (cases S; cases T) auto
+  have \<open>update_flip_watched L ((M, N, br), WL L) ((M', N', br'), WL' L)\<close>
+    using assms(1,2) by (simp add: watch_list_eq)
+  then have \<open>invariant_flipping L ((M', N', br'), WL' L)\<close>
+    by (metis ST(1) assms(2) convert_sls_watch_state_list.simps invariant_wl_flipping_def
+        sls_watch_invariant_update_flip_watched snd_eqD)
+  moreover have \<open>watch (M',N',br',WL') = (\<lambda>L. watched L (convert_sls_watch_state_list (M',N',br',WL')))\<close>
+    using assms unfolding ST
+  proof (induction rule: update_flip_watched_list.induct)
     case (other_true_literal L' C M WL L WL_remaining N br)
     moreover have \<open>L \<noteq> L'\<close>
-      using other_true_literal unfolding invariant_wl_step_def invariant_step_def sls_invariant_def by (auto simp: consistent_interp_def)
+      using other_true_literal unfolding invariant_wl_flipping_def invariant_flipping_def sls_invariant_def by (auto simp: consistent_interp_def)
     then show ?case
       using other_true_literal
-      by (auto intro!: ext simp: invariant_wl_step_def Local_Search_Watch.invariant_step_def)
+      by (auto intro!: ext simp: watched_def invariant_wl_flipping_def 
+          Local_Search_Watch.invariant_flipping_def)
   next
     case (broken_clause C M WL L WL_remaining N br)
     then show ?case 
-      by (auto intro!: ext simp: invariant_wl_step_def Local_Search_Watch.invariant_step_def)
+      by (auto intro!: ext simp: watched_def invariant_wl_flipping_def Local_Search_Watch.invariant_flipping_def)
   qed
   ultimately show ?thesis
-    unfolding invariant_wl_step_def by auto
+    unfolding invariant_wl_flipping_def by auto
 qed
 
 
-lemma rtranclp_sls_invariant_watch_update_wl_list:
-  assumes  \<open>(update_wl_list L)\<^sup>*\<^sup>* S S'\<close> \<open>invariant_wl_step S L\<close>
-  shows \<open>invariant_wl_step S' L\<close> using assms 
-  by (induction rule: rtranclp_induct) (auto dest: update_wl_list_correct)
+lemma rtranclp_sls_watch_invariant_update_flip_watched_list:
+  assumes  \<open>(update_flip_watched_list L)\<^sup>*\<^sup>* S S'\<close> \<open>invariant_wl_flipping L S\<close>
+  shows \<open>invariant_wl_flipping L S'\<close> using assms 
+  by (induction rule: rtranclp_induct) (auto dest: update_flip_watched_list_correct)
 
 
-thm local_search_watch_sls_invariant_watch
+thm watch_local_search_sls_watch_invariant
 
-lemma sls_invariant_watch_list_nostep_update_wl:
-  assumes \<open>invariant_wl_step S L\<close> and \<open>watch S L = {#}\<close>
-  shows \<open>sls_invariant_watch_list S\<close>
-  using assms sls_invariant_watch_nostep_update_wl[of L \<open>convert_sls_state_watch_list S\<close>]
-  unfolding sls_invariant_watch_list_def sls_invariant_watch_def
-  invariant_wl_step_def
+lemma sls_watch_invariant_list_nostep_update_flip_watched:
+  assumes \<open>invariant_wl_flipping L S\<close> and \<open>watch S L = {#}\<close>
+  shows \<open>sls_watch_invariant_list S\<close>
+  using assms sls_watch_invariant_nostep_update_flip_watched[of L \<open>convert_sls_watch_state_list S\<close>]
+  unfolding sls_watch_invariant_list_def sls_watch_invariant_def
+    invariant_wl_flipping_def
   by (cases S) auto
 
-
-text\<open>No time left to finish this lemma, but would work similar to 
-local_search_watch_sls_invariant_watch\<close>
-lemma local_search_watch_list_sls_invariant_watch_list:
-  assumes \<open>local_search_watch_list S T\<close> and \<open>sls_invariant_watch_list S\<close>
-  shows \<open>sls_invariant_watch_list T\<close>
+lemma watch_local_search_list_sls_watch_invariant_list:
+  assumes \<open>watch_local_search_list S T\<close> and \<open>sls_watch_invariant_list S\<close>
+  shows \<open>sls_watch_invariant_list T\<close>
   using assms
-proof (induction rule: local_search_watch_list.induct)
+proof (induction rule: watch_local_search_list.induct)
   case (flip M' M L br1 br N' N WL1 N'' br' WL' WL)
-  have start: \<open>sls_invariant_watch_list (M, N, br, WL)\<close>
-    \<open>sls_invariant_watch (M, N, br)\<close>
-    using flip unfolding sls_invariant_watch_list_def by simp_all 
-  then have step1: \<open>invariant_wl_step (M', N', br1, WL1) L\<close>
-    unfolding invariant_wl_step_def sls_invariant_watch_list_def
-    using sls_invariant_watch_fststep_update_wl[OF start(2), of L] flip
+  have start: \<open>sls_watch_invariant_list (M, N, br, WL)\<close>
+    \<open>sls_watch_invariant (M, N, br)\<close>
+    using flip unfolding sls_watch_invariant_list_def by simp_all 
+  then have step1: \<open>invariant_wl_flipping L (M', N', br1, WL1)\<close>
+    unfolding invariant_wl_flipping_def sls_watch_invariant_list_def
+    using sls_watch_invariant_fststep_update_flip_watched[OF start(2), of L] flip
     apply (auto simp: watched_def filter_mset_empty_conv intro!: ext)
     by (smt (verit) Diff_iff Un_iff add.right_neutral consistent_interp_def
         consistent_interp_single filter_mset_empty_conv filter_mset_eq_conv flip.hyps(1) fst_conv
-        insertCI invariant_step.simps mset_subset_eq_multiset_union_diff_commute snd_conv
+        insertCI invariant_flipping.simps mset_subset_eq_multiset_union_diff_commute snd_conv
         union_iff)
-  then have step3: \<open>invariant_wl_step (M', N'', br', WL') L\<close>
-    using flip.hyps(5) rtranclp_sls_invariant_watch_update_wl_list
+  then have step3: \<open>invariant_wl_flipping L (M', N'', br', WL')\<close>
+    using flip.hyps(5) rtranclp_sls_watch_invariant_update_flip_watched_list
     by blast 
   then show ?case
-    using flip.hyps(8) sls_invariant_watch_list_nostep_update_wl by force
+    using flip.hyps(8) sls_watch_invariant_list_nostep_update_flip_watched by force
 qed
 
 end
